add pow and notation

theories/AD.v
@@ -33,7 +33,7 @@ Theorem real_Ddiv :
     forall x y, real (Ddiv x y) = (real x * inv (real y))%S.
 Proof. intros. unfold Ddiv. rewrite real_mul, real_Dinv. reflexivity. Qed.
 
-(* Single-variable expression language *)
+(* Expression language *)
 Inductive Expr : Set :=
 | Const (s : S)
 | Var   (i : nat)
@@ -41,7 +41,19 @@ Inductive Expr : Set :=
 | Sub   (e1 e2 : Expr)
 | Mul   (e1 e2 : Expr)
 | Opp   (e : Expr)
-| Div   (e1 e2 : Expr).
+| Div   (e1 e2 : Expr)
+| Pow   (e : Expr) (n : nat).
+
+Notation Sq e    := (Mul e e).
+Notation Cube e  := (Mul e (Mul e e)).
+Notation Recip e := (Div (Const 1%S) e).
+
+(* Power on the base field *)
+Fixpoint S_pow (b : S) (n : nat) : S :=
+    match n with
+    | O    => 1%S
+    | Datatypes.S k  => (b * S_pow b k)%S
+    end.
 
 (* Evaluation over the base field *)
 Fixpoint eval (e : Expr) (x : nat -> S) : S :=
@@ -53,9 +65,16 @@ Fixpoint eval (e : Expr) (x : nat -> S) : S :=
     | Mul e1 e2 => (eval e1 x * eval e2 x)%S
     | Opp e1    => (- eval e1 x)%S
     | Div e1 e2 => (eval e1 x / eval e2 x)%S
+    | Pow e1 n  => S_pow (eval e1 x) n
     end.
 
 (* Evaluation over the duals *)
+Fixpoint Dpow (b : D) (n : nat) : D :=
+    match n with
+    | O    => inj 1%S
+    | Datatypes.S k  => Dual.mul b (Dpow b k)
+    end.
+
 Fixpoint eval_dual (e : Expr) (x : nat -> D) : D :=
     match e with
     | Const c   => inj c
@@ -65,51 +84,34 @@ Fixpoint eval_dual (e : Expr) (x : nat -> D) : D :=
     | Mul e1 e2 => Dual.mul (eval_dual e1 x) (eval_dual e2 x)
     | Opp e1    => Dual.opp (eval_dual e1 x)
     | Div e1 e2 => Ddiv (eval_dual e1 x) (eval_dual e2 x)
+    | Pow e1 n  => Dpow (eval_dual e1 x) n
+    end.
+
+(* Derivative of a power by recursion on the exponent
+     (e^{k+1})' = e' * e^k + e * (e^k)' *)
+Fixpoint deriv_pow (de1 e1 : Expr) (n : nat) : Expr :=
+    match n with
+    | O    => Const 0%S
+    | Datatypes.S k => Add (Mul de1 (Pow e1 k)) (Mul e1 (deriv_pow de1 e1 k))
     end.
 
 (* Symbolic derivative *)
-(* Inductive derivative : Expr -> Expr -> Prop :=
-| DConst x    : derivative (Const x) (Const 0%S)
-| DVar        : derivative Var (Const 1%S)
-| DAdd e1  e2
-      de1 de2 :
-    derivative e1 de1 ->
-    derivative e2 de2 ->
-    derivative (Add e1 e2) (Add de1 de2)
-| DSub e1  e2
-      de1 de2 :
-    derivative e1 de1 ->
-    derivative e2 de2 ->
-    derivative (Sub e1 e2) (Sub de1 de2)
-| DMul e1  e2
-      de1 de2 :
-    derivative e1 de1 ->
-    derivative e2 de2 ->
-    derivative (Mul e1 e2) (Add (Mul de1 e2) (Mul e1 de2))
-| DOpp e1 de1 :
-    derivative e1 de1 ->
-    derivative (Opp e1) (Opp de1)
-| DDiv e1  e2
-      de1 de2 :
-    derivative e1 de1 ->
-    derivative e2 de2 ->
-    (forall x, eval e2 x <> 0%S) ->
-    derivative (Div e1 e2)
-        (Div (Sub (Mul de1 e2) (Mul e1 de2)) (Mul e2 e2)). *)
-
+Reserved Notation "'d/dx' e '@' v" (at level 0).
 Fixpoint deriv (e : Expr) (v : nat -> S) : Expr :=
     match e with
     | Const _   => Const 0%S
     | Var j     => Const (v j)
-    | Add e1 e2 => Add (deriv e1 v) (deriv e2 v)
-    | Sub e1 e2 => Sub (deriv e1 v) (deriv e2 v)
-    | Mul e1 e2 => Add (Mul (deriv e1 v) e2) (Mul e1 (deriv e2 v))
-    | Opp e1    => Opp (deriv e1 v)
+    | Add e1 e2 => Add (d/dx e1 @ v) (d/dx e2 @ v)
+    | Sub e1 e2 => Sub (d/dx e1 @ v) (d/dx e2 @ v)
+    | Mul e1 e2 => Add (Mul (d/dx e1 @ v) e2) (Mul e1 (d/dx e2 @ v))
+    | Opp e1    => Opp (d/dx e1 @ v)
     | Div e1 e2 =>
         (* (e1' e2 - e1 e2') / e2^2 *)
-        Div (Sub (Mul (deriv e1 v) e2) (Mul e1 (deriv e2 v)))
+        Div (Sub (Mul (d/dx e1 @ v) e2) (Mul e1 (d/dx e2 @ v)))
             (Mul e2 e2)
-    end.
+    | Pow e1 n => deriv_pow (d/dx e1 @ v) e1 n
+    end
+where "'d/dx' e '@' v" := (deriv e v).
 
 (* Well-definedness: Every denominator is nonzero *)
 Fixpoint defined_at (e : Expr) (x : nat -> S) : Prop :=
@@ -121,19 +123,30 @@ Fixpoint defined_at (e : Expr) (x : nat -> S) : Prop :=
     | Mul e1 e2 => defined_at e1 x /\ defined_at e2 x
     | Opp e1    => defined_at e1 x
     | Div e1 e2 => defined_at e1 x /\ defined_at e2 x /\ (eval e2 x <> 0)%S
+    | Pow e1 _  => defined_at e1 x
     end.
+
+Lemma real_Dpow :
+    forall (d : D) (n : nat),
+        real (Dpow d n) = S_pow (real d) n.
+Proof.
+    intros d n. induction n as [| k IH].
+    - cbn. reflexivity.
+    - cbn. now rewrite <- real_mul, <- IH.
+Qed.
 
 (* Correctness
 
-   Evaluating an expression [e] over multivariate dual numbers gives two results:
-   1. The real part is the standard evaluation of the expression
-   2. The dual part is the partial derivative with respect to variable [i]. *)
+   Evaluating an expression [e] over multivariate dual numbers gives two
+   results:
+   1. The real part is the standard evaluation of the expression.
+   2. The dual part is the seeded derivative [eval (d/dx e @ v) a]. *)
 Theorem eval_dual_correct :
     forall (e : Expr) (a : nat -> S) (v : nat -> S),
         let env : nat -> D := fun j => (a j, v j) in
         defined_at e a ->
         real (eval_dual e env) = eval e a /\
-        du (eval_dual e env)   = eval (deriv e v) a.
+        du (eval_dual e env)   = eval (d/dx e @ v) a.
 Proof.
     induction e; cbv zeta; intros a v Hdef; cbn in Hdef.
     - (* Const c *)
@@ -171,6 +184,15 @@ Proof.
       + unfold Ddiv. rewrite Hr1, Hd1, Hr2, Hd2.
         rewrite div_def.
         field. apply Hnz.
+    - (* Pow e1 n *)
+      destruct (IHe a v Hdef) as [Hr1 Hd1].
+      split.
+      + cbn [eval_dual eval]. rewrite real_Dpow, Hr1. reflexivity.
+      + induction n as [| k IHk].
+        * reflexivity.
+        * cbn [eval_dual Dpow deriv deriv_pow eval] in *.
+          rewrite du_mul, Hr1, Hd1, real_Dpow, Hr1, IHk.
+          ring.
 Qed.
 
 End GDualAD.
